std/latch1 → saturn/spsc_latch1.

theories/saturn/spsc_latch1.v
@@ -6,10 +6,10 @@ From zebre.iris.base_logic Require Import
 From zebre.language Require Import
   notations
   diaframe.
-From zebre.std Require Export
-  base.
 From zebre.std Require Import
   condition.
+From zebre.saturn Require Export
+  base.
 From zebre Require Import
   options.
 
@@ -29,21 +29,21 @@ Implicit Types l : location.
 )(in custom zebre_field
 ).
 
-Definition latch1_create : val :=
+Definition spsc_latch1_create : val :=
   λ: <>,
     let: "t" := { #false; (); () } in
     "t" <-{mutex} mutex_create () ;;
     "t" <-{condition} condition_create () ;;
     "t".
 
-Definition latch1_signal : val :=
+Definition spsc_latch1_signal : val :=
   λ: "t",
     mutex_protect "t".{mutex} (λ: <>,
       "t" <-{flag} #true
     ) ;;
     condition_signal "t".{condition}.
 
-Definition latch1_wait : val :=
+Definition spsc_latch1_wait : val :=
   λ: "t",
     let: "mtx" := "t".{mutex} in
     let: "cond" := "t".{condition} in
@@ -51,99 +51,97 @@ Definition latch1_wait : val :=
       condition_wait_until "cond" "mtx" (λ: <>, "t".{flag})
     ).
 
-Class Latch1G Σ `{zebre_G : !ZebreG Σ} := {
-  #[local] latch1_G_mutex_G :: MutexG Σ ;
-  #[local] latch1_G_producer_G :: OneshotG Σ unit unit ;
-  #[local] latch1_G_consumer_G :: ExclG Σ unitO ;
+Class SpscLatch1G Σ `{zebre_G : !ZebreG Σ} := {
+  #[local] spsc_latch1_G_mutex_G :: MutexG Σ ;
+  #[local] spsc_latch1_G_producer_G :: OneshotG Σ unit unit ;
+  #[local] spsc_latch1_G_consumer_G :: ExclG Σ unitO ;
 }.
 
-Definition latch1_Σ := #[
+Definition spsc_latch1_Σ := #[
   mutex_Σ ;
   oneshot_Σ unit unit ;
   excl_Σ unitO
 ].
-#[global] Instance subG_latch1_Σ Σ `{zebre_G : !ZebreG Σ} :
-  subG latch1_Σ Σ →
-  Latch1G Σ .
+#[global] Instance subG_spsc_latch1_Σ Σ `{zebre_G : !ZebreG Σ} :
+  subG spsc_latch1_Σ Σ →
+  SpscLatch1G Σ .
 Proof.
   solve_inG.
 Qed.
 
-Section latch1_G.
-  Context `{latch1_G : Latch1G Σ}.
+Section spsc_latch1_G.
+  Context `{spsc_latch1_G : SpscLatch1G Σ}.
 
-  Record latch1_meta := {
-    latch1_meta_producer : gname ;
-    latch1_meta_consumer : gname ;
+  Record spsc_latch1_meta := {
+    spsc_latch1_meta_producer : gname ;
+    spsc_latch1_meta_consumer : gname ;
   }.
-  Implicit Types γ : latch1_meta.
+  Implicit Types γ : spsc_latch1_meta.
 
-  #[local] Instance latch1_meta_eq_dec : EqDecision latch1_meta :=
+  #[local] Instance spsc_latch1_meta_eq_dec : EqDecision spsc_latch1_meta :=
     ltac:(solve_decision).
-  #[local] Instance latch1_meta_countable :
-    Countable latch1_meta.
+  #[local] Instance spsc_latch1_meta_countable :
+    Countable spsc_latch1_meta.
   Proof.
     pose encode γ := (
-      γ.(latch1_meta_producer),
-      γ.(latch1_meta_consumer)
+      γ.(spsc_latch1_meta_producer),
+      γ.(spsc_latch1_meta_consumer)
     ).
     pose decode := λ '(γ_producer, γ_consumer), {|
-      latch1_meta_producer := γ_producer ;
-      latch1_meta_consumer := γ_consumer ;
+      spsc_latch1_meta_producer := γ_producer ;
+      spsc_latch1_meta_consumer := γ_consumer ;
     |}.
     refine (inj_countable' encode decode _). intros []. done.
   Qed.
 
-  #[local] Definition latch1_inv_inner l γ P : iProp Σ :=
+  #[local] Definition spsc_latch1_inv_inner l γ P : iProp Σ :=
     ∃ b,
     l.[flag] ↦ #b ∗
     if b then
-      oneshot_shot γ.(latch1_meta_producer) () ∗
-      ( P
-      ∨ excl γ.(latch1_meta_consumer) ()
-      )
+      oneshot_shot γ.(spsc_latch1_meta_producer) () ∗
+      (P ∨ excl γ.(spsc_latch1_meta_consumer) ())
     else
-      oneshot_pending γ.(latch1_meta_producer) (DfracOwn (1/3)) ().
-  #[local] Definition latch1_inv t P : iProp Σ :=
+      oneshot_pending γ.(spsc_latch1_meta_producer) (DfracOwn (1/3)) ().
+  #[local] Definition spsc_latch1_inv t P : iProp Σ :=
     ∃ l γ mtx cond,
     ⌜t = #l⌝ ∗
     meta l nroot γ ∗
     l.[mutex] ↦□ mtx ∗
-    mutex_inv mtx (latch1_inv_inner l γ P) ∗
+    mutex_inv mtx (spsc_latch1_inv_inner l γ P) ∗
     l.[condition] ↦□ cond ∗
     condition_inv cond.
 
-  Definition latch1_producer t : iProp Σ :=
+  Definition spsc_latch1_producer t : iProp Σ :=
     ∃ l γ,
     ⌜t = #l⌝ ∗
     meta l nroot γ ∗
-    oneshot_pending γ.(latch1_meta_producer) (DfracOwn (2/3)) ().
+    oneshot_pending γ.(spsc_latch1_meta_producer) (DfracOwn (2/3)) ().
 
-  Definition latch1_consumer t : iProp Σ :=
+  Definition spsc_latch1_consumer t : iProp Σ :=
     ∃ l γ,
     ⌜t = #l⌝ ∗
     meta l nroot γ ∗
-    excl γ.(latch1_meta_consumer) ().
+    excl γ.(spsc_latch1_meta_consumer) ().
 
-  #[global] Instance latch1_inv_persistent t P :
-    Persistent (latch1_inv t P).
+  #[global] Instance spsc_latch1_inv_persistent t P :
+    Persistent (spsc_latch1_inv t P).
   Proof.
     apply _.
   Qed.
-  #[global] Instance latch1_producer_timeless t :
-    Timeless (latch1_producer t).
+  #[global] Instance spsc_latch1_producer_timeless t :
+    Timeless (spsc_latch1_producer t).
   Proof.
     apply _.
   Qed.
-  #[global] Instance latch1_consumer_timeless t :
-    Timeless (latch1_consumer t).
+  #[global] Instance spsc_latch1_consumer_timeless t :
+    Timeless (spsc_latch1_consumer t).
   Proof.
     apply _.
   Qed.
 
-  Lemma latch1_producer_exclusive t :
-    latch1_producer t -∗
-    latch1_producer t -∗
+  Lemma spsc_latch1_producer_exclusive t :
+    spsc_latch1_producer t -∗
+    spsc_latch1_producer t -∗
     False.
   Proof.
     iIntros "(%l & %γ & -> & #Hmeta & Hpending) (%_l & %_γ & %Heq & _Hmeta & Hpending')". injection Heq as <-.
@@ -151,9 +149,9 @@ Section latch1_G.
     iDestruct (oneshot_pending_valid_2 with "Hpending Hpending'") as %(? & _). done.
   Qed.
 
-  Lemma latch1_consumer_exclusive t :
-    latch1_consumer t -∗
-    latch1_consumer t -∗
+  Lemma spsc_latch1_consumer_exclusive t :
+    spsc_latch1_consumer t -∗
+    spsc_latch1_consumer t -∗
     False.
   Proof.
     iIntros "(%l & %γ & -> & #Hmeta & Hexcl) (%_l & %_γ & %Heq & _Hmeta & Hexcl')". injection Heq as <-.
@@ -161,14 +159,14 @@ Section latch1_G.
     iDestruct (excl_exclusive with "Hexcl Hexcl'") as %[].
   Qed.
 
-  Lemma latch1_create_spec P :
+  Lemma spsc_latch1_create_spec P :
     {{{ True }}}
-      latch1_create ()
+      spsc_latch1_create ()
     {{{ t,
       RET t;
-      latch1_inv t P ∗
-      latch1_producer t ∗
-      latch1_consumer t
+      spsc_latch1_inv t P ∗
+      spsc_latch1_producer t ∗
+      spsc_latch1_consumer t
     }}}.
   Proof.
     iIntros "%Φ _ HΦ".
@@ -181,15 +179,15 @@ Section latch1_G.
     iEval (assert (1 = 2/3 + 1/3)%Qp as -> by compute_done) in "Hpending".
     iDestruct "Hpending" as "(Hpending1 & Hpending2)".
 
-    iMod (excl_alloc (excl_G := latch1_G_consumer_G) ()) as "(%γ_consumer & Hexcl)".
+    iMod (excl_alloc (excl_G := spsc_latch1_G_consumer_G) ()) as "(%γ_consumer & Hexcl)".
 
     pose γ := {|
-      latch1_meta_producer := γ_producer ;
-      latch1_meta_consumer := γ_consumer ;
+      spsc_latch1_meta_producer := γ_producer ;
+      spsc_latch1_meta_consumer := γ_consumer ;
     |}.
     iMod (meta_set _ _ γ nroot with "Hmeta") as "#Hmeta"; first done.
 
-    wp_smart_apply (mutex_create_spec (latch1_inv_inner l γ P) with "[Hflag Hpending2]") as "%mtx #Hmtx_inv"; first iSteps.
+    wp_smart_apply (mutex_create_spec (spsc_latch1_inv_inner l γ P) with "[Hflag Hpending2]") as "%mtx #Hmtx_inv"; first iSteps.
     wp_store.
     iMod (pointsto_persist with "Hmtx") as "Hmtx".
 
@@ -200,13 +198,13 @@ Section latch1_G.
     iSteps.
   Qed.
 
-  Lemma latch1_signal_spec t P :
+  Lemma spsc_latch1_signal_spec t P :
     {{{
-      latch1_inv t P ∗
-      latch1_producer t ∗
+      spsc_latch1_inv t P ∗
+      spsc_latch1_producer t ∗
       P
     }}}
-      latch1_signal t
+      spsc_latch1_signal t
     {{{
       RET (); True
     }}}.
@@ -229,12 +227,12 @@ Section latch1_G.
     iSteps.
   Qed.
 
-  Lemma latch1_wait_spec t P :
+  Lemma spsc_latch1_wait_spec t P :
     {{{
-      latch1_inv t P ∗
-      latch1_consumer t
+      spsc_latch1_inv t P ∗
+      spsc_latch1_consumer t
     }}}
-      latch1_wait t
+      spsc_latch1_wait t
     {{{
       RET ();
       P
@@ -250,7 +248,7 @@ Section latch1_G.
         if b then
           P
         else
-          excl γ.(latch1_meta_consumer) ()
+          excl γ.(spsc_latch1_meta_consumer) ()
       )%I).
       wp_smart_apply (condition_wait_until_spec Ψ with "[$Hcond_inv $Hmtx_inv $Hmtx_locked $Hsignal_inv $Hexcl]").
       { clear. iStep 15 as (Φ b) "Hb Hexcl Hflag".
@@ -262,12 +260,12 @@ Section latch1_G.
     }
     iSteps.
   Qed.
-End latch1_G.
+End spsc_latch1_G.
 
-#[global] Opaque latch1_create.
-#[global] Opaque latch1_wait.
-#[global] Opaque latch1_signal.
+#[global] Opaque spsc_latch1_create.
+#[global] Opaque spsc_latch1_wait.
+#[global] Opaque spsc_latch1_signal.
 
-#[global] Opaque latch1_inv.
-#[global] Opaque latch1_producer.
-#[global] Opaque latch1_consumer.
+#[global] Opaque spsc_latch1_inv.
+#[global] Opaque spsc_latch1_producer.
+#[global] Opaque spsc_latch1_consumer.
